STLC/Basic.lean
@@ -1,0 +1,175 @@
+namespace STLC
+
+inductive Typ
+  | void
+  | unit
+  | sum  (A₁ A₂ : Typ)
+  | prod (A₁ A₂ : Typ)
+  | arr  (A₁ A₂ : Typ)
+
+inductive Ctx
+  | nil
+  | cons (Γ : Ctx) (A : Typ)
+
+inductive Var (A : Typ) : (Γ : Ctx) → Type
+  | zero               : Var A (.cons Γ A)
+  | succ (x : Var A Γ) : Var A (.cons Γ A')
+
+inductive Exp : (Γ : Ctx) → (A : Typ) → Type
+  | var   (x : Var A Γ)                                                              : Exp Γ A
+  | abort (M : Exp Γ .void)                                                          : Exp Γ A
+  | triv                                                                             : Exp Γ .unit
+  | inl   (M : Exp Γ A₁)                                                             : Exp Γ (.sum A₁ A₂)
+  | inr   (M : Exp Γ A₂)                                                             : Exp Γ (.sum A₁ A₂)
+  | case  (M : Exp Γ (.sum A₁ A₂)) (M₁ : Exp (Γ.cons A₁) A) (M₂ : Exp (Γ.cons A₂) A) : Exp Γ A
+  | pair  (M₁ : Exp Γ A₁) (M₂ : Exp Γ A₂)                                            : Exp Γ (.prod A₁ A₂)
+  | prl   (M : Exp Γ (.prod A₁ A₂))                                                  : Exp Γ A₁
+  | prr   (M : Exp Γ (.prod A₁ A₂))                                                  : Exp Γ A₂
+  | lam   (M : Exp (Γ.cons A₁) A₂)                                                   : Exp Γ (.arr A₁ A₂)
+  | ap    (M : Exp Γ (.arr A₁ A₂)) (M₁ : Exp Γ A₁)                                   : Exp Γ A₂
+
+def Renaming (Γ Γ' : Ctx) : Type :=
+  ∀ {{A}}, (x : Var A Γ') → Var A Γ
+
+namespace Renaming
+
+@[simp]
+def cons (γ : Renaming Γ Γ') (y : Var A Γ) : Renaming Γ (Γ'.cons A)
+  | _, .zero   => y
+  | _, .succ x => γ x
+
+@[simp]
+def weaken (γ : Renaming Γ Γ') : Renaming (Γ.cons A) (Γ'.cons A) :=
+  cons (fun _ x => .succ (γ x)) .zero
+
+@[simp]
+def apply (γ : Renaming Γ Γ') : (M : Exp Γ' A) → Exp Γ A
+  | .var x        => .var (γ x)
+  | .abort M      => .abort (γ.apply M)
+  | .triv         => .triv
+  | .inl M        => .inl (γ.apply M)
+  | .inr M        => .inr (γ.apply M)
+  | .case M M₁ M₂ => .case (γ.apply M) (γ.weaken.apply M₁) (γ.weaken.apply M₂)
+  | .pair M₁ M₂   => .pair (γ.apply M₁) (γ.apply M₂)
+  | .prl M        => .prl (γ.apply M)
+  | .prr M        => .prr (γ.apply M)
+  | .lam M        => .lam (γ.weaken.apply M)
+  | .ap M M₁      => .ap (γ.apply M) (γ.apply M₁)
+
+@[simp]
+theorem weaken_id : cons (Γ := .cons Γ A) (fun _ => .succ) .zero = fun _ x => x := by
+  funext _ x
+  cases x
+    <;> simp
+
+@[simp]
+theorem apply_id : apply (fun _ x => x) M = M := by
+  induction M
+    <;> simp [*]
+
+end Renaming
+
+@[simp]
+def Exp.weaken : (M : Exp Γ A) → Exp (Γ.cons A') A :=
+  Renaming.apply fun _ => .succ
+
+def Subst (Γ Γ' : Ctx) : Type :=
+  ∀ {{A}}, (x : Var A Γ') → Exp Γ A
+
+namespace Subst
+
+@[simp]
+def cons (γ : Subst Γ Γ') (M : Exp Γ A) : Subst Γ (Γ'.cons A)
+  | _, .zero   => M
+  | _, .succ x => γ x
+
+@[simp]
+def weaken (γ : Subst Γ Γ') : Subst (Γ.cons A) (Γ'.cons A) :=
+  cons (fun _ x => (γ x).weaken) (.var .zero)
+
+@[simp]
+def apply (γ : Subst Γ Γ') : (M : Exp Γ' A) → Exp Γ A
+  | .var x        => γ x
+  | .abort M      => .abort (γ.apply M)
+  | .triv         => .triv
+  | .inl M        => .inl (γ.apply M)
+  | .inr M        => .inr (γ.apply M)
+  | .case M M₁ M₂ => .case (γ.apply M) (γ.weaken.apply M₁) (γ.weaken.apply M₂)
+  | .pair M₁ M₂   => .pair (γ.apply M₁) (γ.apply M₂)
+  | .prl M        => .prl (γ.apply M)
+  | .prr M        => .prr (γ.apply M)
+  | .lam M        => .lam (γ.weaken.apply M)
+  | .ap M M₁      => .ap (γ.apply M) (γ.apply M₁)
+
+@[simp]
+theorem weaken_var : cons (Γ := .cons Γ A) (fun _ x => .var x.succ) (.var .zero) = fun _ => .var := by
+  funext _ x
+  cases x
+    <;> simp
+
+@[simp]
+theorem apply_var : apply (fun _ => .var) M = M := by
+  induction M
+    <;> simp [*]
+
+theorem cons_renaming (γ : Renaming Γ Γ') (y : Var A Γ) : cons (fun _ x => .var (γ x)) (.var y) = fun _ x => .var (Renaming.cons γ y x) := by
+  funext _ x
+  cases x
+    <;> simp
+
+@[simp]
+theorem apply_renaming (γ : Renaming Γ Γ') : apply (fun _ x => .var (γ x)) M = γ.apply M := by
+  induction M generalizing Γ
+    <;> simp [cons_renaming, *]
+    <;> constructor
+    <;> rfl
+
+end Subst
+
+@[simp]
+def Exp.subst (M : Exp (Γ.cons A') A) (M' : Exp Γ A') : Exp Γ A :=
+  Subst.cons (fun _ => var) M' |>.apply M
+
+@[simp]
+def Exp.subst₁ (M : Exp (.cons Γ A') A) (M' : Exp (Γ.cons A'') A') : Exp (Γ.cons A'') A :=
+  Subst.cons (fun _ x => var x.succ) M' |>.apply M
+
+section
+
+local macro "lemma" M:ident Γ:ident Γ':ident : tactic =>
+  `(tactic|
+    induction $M generalizing $Γ $Γ'
+      <;> simp [*]
+      <;> (try constructor)
+      <;> congr
+      <;> funext _ x
+      <;> cases x
+      <;> simp
+  )
+
+@[simp]
+theorem Renaming.rename_rename (γ : Renaming Γ Γ') (γ' : Renaming Γ' Γ'') : γ.apply (γ'.apply M) = apply (fun A x => γ (γ' x)) M :=
+  by lemma M Γ Γ'
+
+@[simp]
+theorem Subst.subst_rename (γ : Subst Γ Γ') (γ' : Renaming Γ' Γ'') : γ.apply (γ'.apply M) = apply (fun A x => γ (γ' x)) M :=
+  by lemma M Γ Γ'
+
+@[simp]
+theorem Subst.rename_subst (γ : Renaming Γ Γ') (γ' : Subst Γ' Γ'') : γ.apply (γ'.apply M) = apply (fun A x => γ.apply (γ' x)) M :=
+  by lemma M Γ Γ'
+
+@[simp]
+theorem Subst.subst_subst (γ : Subst Γ Γ') (γ' : Subst Γ' Γ'') : γ.apply (γ'.apply M) = apply (fun A x => γ.apply (γ' x)) M :=
+  by lemma M Γ Γ'
+
+end
+
+macro "lemma" : tactic =>
+  `(tactic|
+    simp
+      <;> congr
+      <;> funext _ x
+      <;> cases x
+      <;> simp
+  )
