lakefile.lean
@@ -6,5 +6,7 @@ package common
 @[default_target]
 lean_lib Common
 
+lean_lib STLC
+
 require mathlib from git "https://github.com/leanprover-community/mathlib4.git"
 require rec from "rec"
